high2/Zeta.EAC.fst
@@ -1,0 +1,29 @@
+module Zeta.EAC
+
+open Zeta.SeqAux
+
+let eac_implies_prefix_eac
+  (#app: app_params)
+  (l: eac_log app)
+  (i: nat {i <= length l})
+  : Lemma (ensures (eac (prefix l i)))
+  =
+
+  admit()
+
+let max_eac_prefix
+  (#app: app_params)
+  (l:vlog_ext app)
+  : (i:nat{eac l /\ i = length l
+          \/
+          i < length l /\
+          eac (prefix l i) /\
+          ~ (eac (prefix l (i + 1)))})
+  = admit()
+
+(* computable version of eac *)
+let is_eac_log (#app: app_params) (l:vlog_ext app): (r:bool{r <==> eac l})
+  = let i = max_eac_prefix l in
+    if i = length l
+    then true
+    else false
